Circuits.v
@@ -19,7 +19,7 @@ Section Circuit.
   Context {R: reg_t -> nat}.
   Context {Sigma: fn_t -> CExternalSignature}.
 
-  Inductive circuit : nat -> Type :=
+  Inductive circuit {Rwdata} : nat -> Type :=
   | CNot (c: circuit 1): circuit 1
   | CAnd (c1 c2: circuit 1): circuit 1
   | COr (c1 c2: circuit 1): circuit 1
@@ -30,10 +30,12 @@ Section Circuit.
               (a1: circuit (Sigma idx).(arg1Size))
               (a2: circuit (Sigma idx).(arg2Size))
     : circuit (Sigma idx).(retSize)
+  | CBundle {T} (s: T) (bundle: forall (r:reg_t), Rwdata (R r)) : circuit 0
+  | CBundleRef {T sz} (source_bundle: circuit 0) (field:T) (c: circuit sz) : circuit sz
   | CAnnot {sz} (annot: string) (c: circuit sz) : circuit sz.
 End Circuit.
 
-Arguments circuit {reg_t fn_t} R Sigma sz.
+Arguments circuit {reg_t fn_t} R Sigma Rwdata sz.
 
 Section Interpretation.
   Context {reg_t fn_t: Type}.
@@ -43,9 +45,12 @@ Section Interpretation.
   Context {REnv: Env reg_t}.
 
   Context (r: REnv.(env_t) (fun idx => bits (R (idx)))).
+
   Context (sigma: forall f, CExternalSignature_denote (Sigma f)).
 
-  Fixpoint interp_circuit {n} (c: circuit R Sigma n) : bits n :=
+  Context {Rwdata: nat -> Type}.
+
+  Fixpoint interp_circuit {n} (c: circuit R Sigma Rwdata n) : bits n :=
     match c with
     | CNot c =>
       Ob~(negb (Bits.single (interp_circuit c)))
@@ -62,6 +67,10 @@ Section Interpretation.
       REnv.(getenv) r idx
     | CExternal idx arg1 arg2 =>
       sigma idx (interp_circuit arg1) (interp_circuit arg2)
+    | CBundle _ _ =>
+      Ob
+    | CBundleRef _ _ c =>
+      interp_circuit c
     | CAnnot _ c =>
       interp_circuit c
     end.
@@ -69,11 +78,15 @@ End Interpretation.
 
 Section CircuitOptimizer.
   Context {reg_t fn_t: Type}.
+
   Context {R: reg_t -> nat}.
   Context {Sigma: fn_t -> CExternalSignature}.
 
+
+  Context {Rwdata: nat -> Type}.
+
   Notation Circuit := circuit.
-  Notation circuit := (circuit R Sigma).
+  Notation circuit := (circuit R Sigma Rwdata).
 
   Context {REnv: Env reg_t}.
 
@@ -105,7 +118,7 @@ Section CircuitOptimizer.
     match c return option (list bool) with
     | CAnnot annot c =>
       asconst c
-    | @CConst _ _ _ _ sz cst =>
+    | @CConst _ _ _ _ _ sz cst =>
       Some (vect_to_list cst)
     | c => None
     end.
@@ -115,8 +128,9 @@ Section CircuitOptimizer.
 
   Instance EqDec_ListBool : EqDec (list bool) := _.
 
+
   Definition simplify_bool_1' {sz} (c: circuit sz): circuit sz :=
-    match c in Circuit _ _ sz return circuit sz with
+    match c in Circuit _ _ _ sz return circuit sz with
     | (CNot c) as c0 =>
       match asconst c with
       | Some ltrue => CConst Ob~0
@@ -225,11 +239,11 @@ Section CircuitOptimizer.
     {| lco_fn := @simplify_bool_1; lco_proof := @simplify_bool_1_correct |}.
 End CircuitOptimizer.
 
-Arguments simplify_bool_1 {_ _ _ _} [_] _.
-Arguments lco_fn {_ _ _ _ _ _ _} _ {_}.
-Arguments lco_proof {_ _ _ _ _ _ _} _ {_}.
-Arguments lco_compose {_ _ _ _ _ _ _} _ _.
-Arguments bool_simpl_lco {_ _ _ _ _ _ _}.
+Arguments simplify_bool_1 {_ _ _ _ _} [_] _.
+Arguments lco_fn {_ _ _ _ _ _ _ _} _ {_}.
+Arguments lco_proof {_ _ _ _ _ _ _ _} _ {_}.
+Arguments lco_compose {_ _ _ _ _ _ _ _} _ _.
+Arguments bool_simpl_lco {_ _ _ _ _ _ _ _}.
 
 Section CircuitCompilation.
   Context {name_t var_t reg_t fn_t: Type}.
@@ -242,12 +256,18 @@ Section CircuitCompilation.
   Definition CR idx :=
     type_sz (R idx).
 
-  Definition CSigma fn :=
-    {| arg1Size := type_sz (Sigma fn).(arg1Type);
-       arg2Size := type_sz (Sigma fn).(arg2Type);
-       retSize := type_sz (Sigma fn).(retType) |}.
+  Definition CSigma fn := CExternalSignature_of_ExternalSignature (Sigma fn).
 
-  Notation circuit := (circuit CR CSigma).
+  Notation circuit' := (circuit CR CSigma).
+
+  Inductive rwdata {sz: nat} :=
+    { read0: circuit' (@rwdata) 1;
+      read1: circuit' (@rwdata) 1;
+      write0: circuit' (@rwdata) 1;
+      write1: circuit' (@rwdata) 1;
+      data0: circuit' (@rwdata) sz;
+      data1: circuit' (@rwdata) sz }.
+  Notation circuit := (circuit' (@rwdata)).
 
   Context (opt: forall {sz}, circuit sz -> circuit sz).
   Context (r: REnv.(env_t) (fun reg => circuit (CR reg))).
@@ -284,16 +304,9 @@ Section CircuitCompilation.
 
   Local Open Scope circuit.
 
+
   Definition readRegisters : forall idx: reg_t, circuit (CR idx) :=
     fun idx => CReadRegister (R := CR) (Sigma := CSigma) idx.
-
-  Record rwdata {sz} :=
-    { read0: circuit 1;
-      read1: circuit 1;
-      write0: circuit 1;
-      write1: circuit 1;
-      data0: circuit sz;
-      data1: circuit sz }.
 
   Definition rwset :=
     REnv.(env_t) (fun reg => @rwdata (CR reg)).
@@ -485,6 +498,31 @@ Section CircuitCompilation.
 
   Context (rules: name_t -> rule var_t R Sigma).
 
+  Inductive Field := R0 | R1 | W0 | W1 | Data0 | Data1 | CanFire.
+
+  Definition annotate_registers :=
+    (fun bundle_ref =>
+       REnv.(map) (fun r ruleReg =>
+                     {|
+                       read0 := CBundleRef bundle_ref R0 (ruleReg.(read0));
+                       read1 := CBundleRef bundle_ref R1 (ruleReg.(read1));
+                       write0 := CBundleRef bundle_ref W0 (ruleReg.(write0));
+                       write1 := CBundleRef bundle_ref W1 (ruleReg.(write1));
+                       data0 := CBundleRef bundle_ref Data0 (ruleReg.(data0));
+                       data1 := CBundleRef bundle_ref Data1 (ruleReg.(data1))
+                     |} : @rwdata (CR r))).
+
+  Definition annotate_bundle := (fun {sz} bundle_ref (rl: @action_circuit sz)  =>
+    {| canFire := CBundleRef bundle_ref CanFire rl.(erwc).(canFire);
+       regs := annotate_registers bundle_ref ((rl.(erwc)).(regs));
+    |}).
+
+  Definition bundle_rule {tau} (input: rwcircuit) (rl: @action_circuit tau) (rl_name: name_t) :
+    @action_circuit tau :=
+    let bundle_ref := CBundle rl_name (REnv.(getenv) (input.(regs))) in
+    {| erwc:= annotate_bundle bundle_ref rl;
+          retVal:= rl.(retVal) |}.
+
   Fixpoint compile_scheduler'
            (s: scheduler name_t)
            (input: scheduler_circuit):
@@ -492,8 +530,9 @@ Section CircuitCompilation.
     match s with
     | Done =>
       input
-    | Cons rl s =>
-      let (rl, Gamma) := compile_action CtxEmpty (rules rl) (adapter input) in
+    | Cons rl_name s =>
+      let (rl, Gamma) := compile_action CtxEmpty (rules rl_name) (adapter input) in
+      let rl := bundle_rule (adapter input) rl rl_name in
       let acc := update_accumulated_rwset rl.(erwc).(regs) input in
       let will_fire := willFire_of_canFire rl.(erwc) input in
       let input := mux_rwsets "mux_input" will_fire acc input in
